*** empty log message ***

doc-src/TutorialI/Datatype/Nested.thy
@@ -63,7 +63,7 @@ strengthened and proved as follows:
 
 lemma "subst  Var t  = (t ::('a,'b)term)  \\<and>
         substs Var ts = (ts::('a,'b)term list)";
-by(induct_tac t and ts, auto);
+by(induct_tac t and ts, simp_all);
 
 text{*\noindent
 Note that \isa{Var} is the identity substitution because by definition it
@@ -102,50 +102,24 @@ suggested equation holds:
 *}
 
 lemma [simp]: "subst s (App f ts) = App f (map (subst s) ts)"
-by(induct_tac ts, auto)
+by(induct_tac ts, simp_all)
 
-text{*
+text{*\noindent
 What is more, we can now disable the old defining equation as a
 simplification rule:
 *}
 
 lemmas [simp del] = subst_App
 
-text{*
-The advantage is that now we have replaced @{term"substs"} by @{term"map"},
-we can profit from the large number of pre-proved lemmas about @{term"map"}.
-We illustrate this with an example, reversing terms:
-*}
-
-consts trev  :: "('a,'b)term => ('a,'b)term"
-       trevs :: "('a,'b)term list => ('a,'b)term list"
-primrec   "trev (Var x) = Var x"
-trev_App: "trev (App f ts) = App f (trevs ts)"
-
-          "trevs [] = []"
-          "trevs (t#ts) = trevs ts @ [trev t]"
-
 text{*\noindent
-Following the above methodology, we re-express \isa{trev\_App}:
-*}
-
-lemma [simp]: "trev (App f ts) = App f (rev(map trev ts))"
-by(induct_tac ts, auto)
-lemmas [simp del] = trev_App
-
-text{*\noindent
-Now it becomes quite easy to prove @{term"trev(trev t) = t"}, except that we
-still have to come up with the second half of the conjunction:
-*}
-
-lemma "trev(trev t) = (t::('a,'b)term) &
-        map trev (map trev ts) = (ts::('a,'b)term list)";
-by(induct_tac t and ts, auto simp add:rev_map);
-
-text{*\noindent
-Getting rid of this second conjunct requires deriving a new induction schema
-for \isa{term}, which is beyond what we have learned so far. Please stay
-tuned, we will solve this final problem in \S\ref{sec:der-ind-schemas}.
+The advantage is that now we have replaced @{term"substs"} by
+@{term"map"}, we can profit from the large number of pre-proved lemmas
+about @{term"map"}.  Unfortunately inductive proofs about type
+\isa{term} are still awkward because they expect a conjunction. One
+could derive a new induction principle as well (see
+\S\ref{sec:derive-ind}), but turns out to be simpler to define
+functions by \isacommand{recdef} instead of \isacommand{primrec}.
+The details are explained in \S\ref{sec:advanced-recdef} below.
 
 Of course, you may also combine mutual and nested recursion. For example,
 constructor \isa{Sum} in \S\ref{sec:datatype-mut-rec} could take a list of
